#### P6 5 设$a,b$为常数，且$\lim_{x\to\infin}(\sqrt[3]{1-x^6}-ax^2-b)=0$，则$a=$，$b=$

移项取反，
$$
\lim_{x\to\infin}(\sqrt[3]{x^6-1}+ax^2)=-b
$$


**法一**	根据泰勒展开$(1+x)^{\alpha}=1+\alpha x+\frac{\alpha(\alpha-1)}{2!}x^2+...+\frac{\alpha(\alpha-1)...(\alpha-n+1)}{n!}+o(x^n)$

当$x\to\infin$，
$$
\sqrt[3]{x^6-1}=x^2\sqrt[3]{1-\frac{1}{x^6}}=x^2(1-\frac{1}{3x^6}+o(-\frac{1}{x^6}))
$$
则，
$$
\lim_{x\to\infin}x^2(1+a-\frac{1}{3x^6}+o(-\frac{1}{x^6}))=-b
$$
极限要为$\infin×0$，才能等于一个常数，所以$a=-1$，此时
$$
\lim_{x\to\infin}-\frac{1}{3x^4}=0=-b
$$
所以$b=0$

**法二**	倒代换，令$x=\frac{1}{t}$，$t\to0$
$$
\lim_{t\to0}\frac{\sqrt[3]{1-t^6}+a}{t^2}=-b
$$
分子$\to0$，则分母也要$\to0$，即$a=-1$，此时
$$
\lim_{t\to0}\frac{\sqrt[3]{1-t^6}-1}{t^2}=\lim_{t\to0}\frac{-\frac{1}{3}t^6}{t^2}=0=-b
$$
所以$b=0$

**法三**	提项，显然提$x^2$
$$
\lim_{x\to\infin}x^2(\sqrt[3]{1-\frac{1}{x^6}}+a)
$$
极限要为$\infin×0$，才能等于一个常数，所以$a=-1$，此时
$$
\lim_{x\to\infin}x^2(-\frac{1}{3x^6})=-\lim_{x\to\infin}\frac{1}{3x^4}=0=-b
$$
所以$b=0$

